some cleanup

Test/civl/reserve.bpl
@@ -1,36 +1,47 @@
 // RUN: %parallel-boogie "%s" > "%t"
 // RUN: %diff "%s.expect" "%t"
 
+/*
+This example models a memory allocator based on count of free cells (freeSpace) and an
+array that keeps tracks of the allocation status of each cell (isFree). To allocate
+a cell, freeSpace is decremented atomically, blocking to ensure that freeSpace does not
+go below zero. If the decrement succeeds, then a scan of isFree is performed to find a
+free cell. The goal of the verification is to prove that this scan will succeed. The
+main challenge in the proof is to reason about cardinality of constructed sets.
+*/
+
 type {:linear "tid"} Tid = int;
 
 const memLo: int;
 const memHi: int;
 axiom 0 < memLo && memLo <= memHi;
-function memAddr(i: int) returns (bool) { memLo <= i && i < memHi }
+function {:inline} memAddr(i: int) returns (bool) { memLo <= i && i < memHi }
 
 type {:datatype} Bijection;
 function {:constructor} Bijection(domain: [Tid]bool, range: [int]bool, tidToPtr: [Tid]int, ptrToTid: [int]Tid): Bijection;
 
-var {:layer 0,1} Free: [int]bool;
+var {:layer 0,1} isFree: [int]bool;
 var {:layer 0,1} freeSpace: int;
 var {:layer 0,1} allocMap: Bijection;
 
-function BijectionInvariant(allocMap: Bijection): bool {
-    (forall tid: Tid :: domain#Bijection(allocMap)[tid] ==>
-                        range#Bijection(allocMap)[tidToPtr#Bijection(allocMap)[tid]] &&
-                        ptrToTid#Bijection(allocMap)[tidToPtr#Bijection(allocMap)[tid]] == tid)
+function {:inline} BijectionInvariant(allocMap: Bijection): bool {
+    (forall tid: Tid ::
+        domain#Bijection(allocMap)[tid] ==>
+            range#Bijection(allocMap)[tidToPtr#Bijection(allocMap)[tid]] &&
+            ptrToTid#Bijection(allocMap)[tidToPtr#Bijection(allocMap)[tid]] == tid)
     &&
-    (forall ptr: int :: range#Bijection(allocMap)[ptr] ==>
-                        domain#Bijection(allocMap)[ptrToTid#Bijection(allocMap)[ptr]] &&
-                        tidToPtr#Bijection(allocMap)[ptrToTid#Bijection(allocMap)[ptr]] == ptr)
+    (forall ptr: int ::
+        range#Bijection(allocMap)[ptr] ==>
+            domain#Bijection(allocMap)[ptrToTid#Bijection(allocMap)[ptr]] &&
+            tidToPtr#Bijection(allocMap)[ptrToTid#Bijection(allocMap)[ptr]] == ptr)
 }
 
 procedure {:yield_invariant} {:layer 1} YieldInvariant();
 requires 0 <= freeSpace;
 requires BijectionInvariant(allocMap);
-requires (forall y: int :: Free[y] ==> memAddr(y));
-requires MapDiff(range#Bijection(allocMap), Free) == MapConst(false);
-requires freeSpace == Size(MapDiff(Free, range#Bijection(allocMap)));
+requires (forall y: int :: isFree[y] ==> memAddr(y));
+requires MapDiff(range#Bijection(allocMap), isFree) == MapConst(false);
+requires freeSpace == Size(MapDiff(isFree, range#Bijection(allocMap)));
 
 function Size<T>([T]bool) returns (int);
 
@@ -49,8 +60,8 @@ modifies freeSpace, allocMap;
     var ptr: int;
     assume 0 < freeSpace;
     assert !domain#Bijection(allocMap)[tid];
-    assert freeSpace == Size(MapDiff(Free, range#Bijection(allocMap)));
-    assume MapDiff(Free, range#Bijection(allocMap))[ptr];
+    assert freeSpace == Size(MapDiff(isFree, range#Bijection(allocMap)));
+    assume MapDiff(isFree, range#Bijection(allocMap))[ptr];
     freeSpace := freeSpace - 1;
     call allocMap := Reserve(allocMap, tid, ptr);
 }
@@ -69,16 +80,16 @@ procedure {:atomic} Reserve(allocMap: Bijection, tid: Tid, ptr: int) returns (al
 procedure {:yields} {:layer 0} {:refines "atomic_AllocIfPtrFree"} AllocIfPtrFree({:linear "tid"} tid: Tid, ptr: int) returns (spaceFound:bool);
 
 procedure {:atomic} {:layer 1} atomic_AllocIfPtrFree({:linear "tid"} tid: Tid, ptr: int) returns (spaceFound:bool)
-modifies Free, allocMap;
+modifies isFree, allocMap;
 {
     var tid': Tid;
     var ptr': int;
     assert memAddr(ptr);
-    assert Free[ptr] || memAddr(ptr + 1);
+    assert isFree[ptr] || memAddr(ptr + 1);
     assert domain#Bijection(allocMap)[tid];
-    spaceFound := Free[ptr];
+    spaceFound := isFree[ptr];
     if (spaceFound) {
-        Free[ptr] := false;
+        isFree[ptr] := false;
         call allocMap := Alloc(allocMap, tid, ptr);
     }
 }
@@ -110,11 +121,11 @@ procedure {:atomic} Alloc(allocMap: Bijection, tid: Tid, ptr: int) returns (allo
 procedure {:yields} {:layer 0} {:refines "atomic_Reclaim"} Reclaim() returns (ptr: int);
 
 procedure {:atomic} {:layer 1} atomic_Reclaim() returns (ptr: int)
-modifies freeSpace, Free;
+modifies freeSpace, isFree;
 {
-    assume memAddr(ptr) && !Free[ptr];
+    assume memAddr(ptr) && !isFree[ptr];
     freeSpace := freeSpace + 1;
-    Free[ptr] := true;
+    isFree[ptr] := true;
 }
 
 procedure {:yields} {:layer 1}
@@ -128,20 +139,19 @@ requires {:layer 1} !domain#Bijection(allocMap)[tid];
 
     call DecrementFreeSpace(tid);
     i := memLo;
-    call {:layer 1} SizeLemma1(MapDiff(Free, range#Bijection(allocMap)), tidToPtr#Bijection(allocMap)[tid]);
+    call {:layer 1} SizeLemma1(MapDiff(isFree, range#Bijection(allocMap)), tidToPtr#Bijection(allocMap)[tid]);
     while (i < memHi)
-    invariant {:yields} {:layer 1} memAddr(i) && domain#Bijection(allocMap)[tid];
-    invariant {:yields} {:layer 1} i <= tidToPtr#Bijection(allocMap)[tid];
+    invariant {:yields} {:layer 1} memAddr(i) && domain#Bijection(allocMap)[tid] && i <= tidToPtr#Bijection(allocMap)[tid];
     invariant {:yields} {:layer 1} {:yield_loop "YieldInvariant"} true;
     {
-        call {:layer 1} SizeLemma1(Free, i);
+        call {:layer 1} SizeLemma1(isFree, i);
         call {:layer 1} SizeLemma1(range#Bijection(allocMap), i);
         call {:layer 1} SizeLemma1(range#Bijection(allocMap), tidToPtr#Bijection(allocMap)[tid]);
-        call {:layer 1} SizeLemma2(range#Bijection(allocMap), Free);
+        call {:layer 1} SizeLemma2(range#Bijection(allocMap), isFree);
         call spaceFound := AllocIfPtrFree(tid, i);
         if (spaceFound)
         {
-            call {:layer 1} SizeLemma2(range#Bijection(allocMap), Free);
+            call {:layer 1} SizeLemma2(range#Bijection(allocMap), isFree);
             return;
         }
         i := i + 1;
@@ -160,6 +170,6 @@ Collect()
     invariant {:yields} {:layer 1} {:yield_loop "YieldInvariant"} true;
     {
         call ptr := Reclaim();
-        call {:layer 1} SizeLemma1(MapDiff(Free, range#Bijection(allocMap)), ptr);
+        call {:layer 1} SizeLemma1(MapDiff(isFree, range#Bijection(allocMap)), ptr);
     }
 }
